theories/Closed.v
@@ -33,7 +33,7 @@ match t with
   (andb (is_closedn n x)
   (andb (is_closedn (S (S n)) P)
     (andb (is_closedn n hr) (andb (is_closedn n y) (is_closedn n e)))))
-| tQuote t => is_closedn n t
+| tQuote A t => andb (is_closedn n A) (is_closedn n t)
 | tStep t u => andb (is_closedn n t) (is_closedn n u)
 | tReflect t u => andb (is_closedn n t) (is_closedn n u)
 end.
