theories/DeclarativeTyping.v
@@ -128,9 +128,10 @@ Section Definitions.
     [Γ |- y : A] ->
     [Γ |- e : tId A x y] ->
     [Γ |- tIdElim A x P hr y e : P[e .: y..]]
-  | wfTermQuote {Γ} {t} :
-    [Γ |- t ≅ t : arr tNat tNat] ->
-    [Γ |- tQuote t : tNat]
+  | wfTermQuote {Γ} {A t} :
+    [Γ |- A] ->
+    [Γ |- t ≅ t : A] ->
+    [Γ |- tQuote A t : tNat]
   | wfTermStep {Γ} {t u} :
     [Γ |- t ≅ t : arr tNat tNat] ->
     [Γ |- u ≅ u : tNat] ->
@@ -183,13 +184,16 @@ Section Definitions.
     [Γ ,, A |- t : B] ->
     [Γ |- a : A] ->
     [Γ |- tApp (tLambda A t) a ≅ t[a..] : B[a..]]
-  | TermQuoteRed {Γ} {t} :
-    [Γ |- t ≅ t : arr tNat tNat] ->
+  | TermQuoteRed {Γ} {A} {t} :
+    [Γ |- A] ->
+    [Γ |- t ≅ t : A] ->
     dnf t -> closed0 t ->
-    [Γ |- tQuote t ≅ qNat (quote (erase t)) : tNat]
-  | TermQuoteCong {Γ} {t t'} :
-    [Γ |- t ≅ t' : arr tNat tNat] ->
-    [Γ |- tQuote t ≅ tQuote t' : tNat]
+    [Γ |- tQuote A t ≅ qNat (quote (erase t)) : tNat]
+  | TermQuoteCong {Γ} {A A'} {t t'} :
+    [Γ |- A] ->
+    [Γ |- A ≅ A'] ->
+    [Γ |- t ≅ t' : A] ->
+    [Γ |- tQuote A t ≅ tQuote A' t' : tNat]
   | TermStepRed {Γ} {t u k v} :
     [Γ |- t ≅ t : arr tNat tNat] ->
     [Γ |- run : arr tNat (arr tNat tPNat)] ->
